state a local retag lemma

theories/sim/cmra.v
@@ -296,8 +296,11 @@ Proof. intros Eq. rewrite lookup_core Eq /core /= core_id //. Qed.
 
 (** Resources that we own. *)
 
+Definition res_tag tg tk h : resUR :=
+  ({[tg := (to_tagKindR tk, to_agree <$> h)]}, ε, ε).
+
 Definition res_callState (c: call_id) (cs: call_state) : resUR :=
-  ((ε, {[c := to_callStateR cs]}), ε).
+  (ε, {[c := to_callStateR cs]}, ε).
 
 Definition res_mapsto l s stk : resUR :=
-  (ε, {[ l := to_locStateR (lsLocal s stk)]}).
+  (ε, ε, {[ l := to_locStateR (lsLocal s stk)]}).
