theories/sim/simple.v
@@ -115,12 +115,31 @@ Proof.
   intros HH σs σt <-<-. apply sim_body_alloc_local=>/=. eauto.
 Qed.
 
-(* FIXME notation is so broken, can one write this down without the Val? *)
 Lemma sim_simple_write_local fs ft r r' n l tg Ts Tt v v' css cst Φ :
   r ≡ r' ⋅ res_mapsto l v' (init_stack (Tagged tg)) →
   (∀ s, v = [s] → Φ (r' ⋅ res_mapsto l s (init_stack (Tagged tg))) n (ValR [☠%S]) css (ValR [☠%S]) cst) →
   r ⊨ˢ{n,fs,ft}
     (Place l (Tagged tg) Ts <- #v, css) ≥ (Place l (Tagged tg) Tt <- #v, cst)
+  : Φ.
+Proof.
+Admitted.
+
+Lemma sim_simple_retag_local fs ft r r' r'' rf n l s' s tg m ty css cst Φ :
+  r ≡ r' ⋅ res_mapsto l s (init_stack (Tagged tg)) →
+  arel rf s' s →
+  r' ≡ r'' ⋅ rf →
+  (∀ l_inner tg_inner hplt,
+    let s := ScPtr l_inner (Tagged tg_inner) in
+    let tk := match m with Mutable => tkUnique | Immutable => tkPub end in
+    match m with 
+    | Mutable => is_Some (hplt !! l_inner)
+    | Immutable => if is_freeze ty then is_Some (hplt !! l_inner) else True
+    end →
+    Φ (r' ⋅ res_mapsto l s (init_stack (Tagged tg)) ⋅ res_tag tg_inner tk hplt) n (ValR [☠%S]) css (ValR [☠%S]) cst) →
+  r ⊨ˢ{n,fs,ft}
+    (Retag (Place l (Tagged tg) (Reference (RefPtr m) ty)) Default, css)
+  ≥
+    (Retag (Place l (Tagged tg) (Reference (RefPtr m) ty)) Default, cst)
   : Φ.
 Proof.
 Admitted.
